proof/crefine/AARCH64/Delete_C.thy
@@ -894,10 +894,9 @@ lemma finaliseSlot_ccorres:
          apply (clarsimp simp: cte_wp_at_ctes_of)
          apply (erule disjE[where P="F \<and> G" for F G])
           apply (clarsimp simp: capRemovable_def cte_wp_at_ctes_of cap_has_cleanup'_def
+                                cleanup_info_wf'_def arch_cleanup_info_wf'_def Kernel_C_maxIRQ
                          split: option.split capability.splits)
-          apply (auto dest!: ctes_of_valid'
-                       simp: valid_cap'_def Kernel_C.maxIRQ_def AARCH64.maxIRQ_def
-                             unat_ucast word_le_nat_alt cleanup_info_wf'_def arch_cleanup_info_wf'_def)[1]
+          apply (auto dest!: ctes_of_valid' simp: valid_cap'_def word_le_nat_alt)[1]
          subgoal by (auto dest!: valid_capAligned ctes_of_valid'
                           simp: isCap_simps final_matters'_def o_def)
         apply clarsimp
