proof/crefine/AARCH64/Wellformed_C.thy
@@ -541,6 +541,27 @@ lemma num_tcb_queues_calculation:
   "num_tcb_queues = numDomains * numPriorities"
   unfolding num_tcb_queues_val by eval
 
+text \<open>maxIRQ interface\<close>
+
+(* Main lemma to use when one encounters Kernel_C.maxIRQ *)
+lemma Kernel_C_maxIRQ:
+  "Kernel_C.maxIRQ = Kernel_Config.maxIRQ"
+  by (simp add: Kernel_C.maxIRQ_def Kernel_Config.maxIRQ_def)
+
+value_type irq_array_size = "Suc Kernel_Config.maxIRQ"
+
+(* For numeral array guard assertions. *)
+lemma unat_irq_array_guard[unfolded irq_array_size_val, simplified]:
+  "unat irq \<le> Kernel_Config.maxIRQ \<Longrightarrow> unat irq < irq_array_size" for irq::irq
+  by (simp add: irq_array_size_def)
+
+lemma ucast_irq_array_guard[unfolded irq_array_size_val, simplified]:
+  "irq \<le> Kernel_Config.maxIRQ \<Longrightarrow> ucast irq < (of_nat irq_array_size :: machine_word)" for irq::irq
+  apply (simp add: irq_array_size_def word_less_nat_alt word_le_nat_alt)
+  apply (rule order_le_less_trans, rule unat_ucast_le)
+  apply simp
+  done
+
 
 (* Input abbreviations for API object types *)
 (* disambiguates names *)
